src/util/Autodestr.v
@@ -1,10 +1,19 @@
 (*https://github.com/mit-plv/fiat-crypto/blob/master/src/Util/Tactics/DestructHyps.v ?*)
 From coqutil Require Import Ltac2.
-Ltac2 mutable to_destruct () : constr list := [].
-Ltac2 Set to_destruct as old_to_destruct := fun _ => constr:(prod nat nat) :: old_to_destruct ().
+Ltac2 mutable to_destruct () : (constr -> bool) list := [].
+Ltac2 boolify (tac : unit -> 'a) : bool :=
+  match Control.case tac with
+  | Err _ => false
+  | Val (_, _) => true
+  end.
+Ltac2 Check boolify.
 
-Ltac2 Check destruct0.
-Print Std.induction_clause.
+Ltac2 Check Pattern.matches.
+Ltac2 Eval Pattern.matches pat:(?x) constr:(nat).
+Ltac2 pattern_pred p c := boolify (fun _ => Pattern.matches p c).
+
+Ltac2 Set to_destruct as to_destruct' := fun _ => pattern_pred pat:(prod _ _) :: to_destruct' ().
+
 Ltac2 y () := destruct z, w.
 Print Ltac2 y.
 Ltac2 simple_induction_clause (id : ident) : Std.induction_clause :=
@@ -14,12 +23,13 @@ Ltac2 simple_induction_clause (id : ident) : Std.induction_clause :=
     Std.indcl_in := None; }.
 
 Ltac2 simple_destruct (ids : ident list) :=
-  destruct0 false (List.map simple_induction_clause ids) (fun _ => None).
+  match ids with
+  | [] => ()
+  | _ :: _ => destruct0 false (List.map simple_induction_clause ids) (fun _ => None)
+  end.
 
-Ltac2 Check Control.hyps.
-Ltac2 Check List.exist.
-Ltac2 matching_hyps (ts : constr list) :=
-  List.filter (fun (_, _, t) => List.exist (Constr.equal t) ts) (Control.hyps ()).
+Ltac2 matching_hyps (ts : (constr -> bool) list) :=
+  List.filter (fun (_, _, t) => List.exist (fun test => test t) ts) (Control.hyps ()).
 
 Ltac2 matching_hyp_ids ts :=
   List.map (fun (name, _, _) => name) (matching_hyps ts).
@@ -30,11 +40,9 @@ Ltac2 destruct_matching_hyps ts :=
 Ltac2 autodestr0 () := destruct_matching_hyps (to_destruct ()).
 
 Ltac2 Notation autodestr := autodestr0 ().
-Ltac2 Eval matching_hyp_ids (to_destruct ()).
-
+Ltac autodestr := ltac2:(autodestr).
 Goal forall x : nat * nat, nat.
-  Ltac2 Eval matching_hyp_ids (to_destruct ()).
-  intros.
-  Ltac2 Eval matching_hyp_ids (to_destruct ()).
-  Ltac2 Eval Control.hyps ().
   autodestr.
+  intros.
+  autodestr.
+Abort.
